src/CFG/CFG_Transfer.thy
@@ -20,6 +20,7 @@ lemma edge_collect_simps [simp]:
   "edge_collect (EA_AssumeNot b) S = {s. s \<in> S \<and> \<not> bval b s}"
   "edge_collect (EA_Ret e p) S =
      {s(ret_var := (case e of None \<Rightarrow> s ret_var | Some a \<Rightarrow> aval a s)) | s. s \<in> S}"
+  "edge_collect (EA_Check c) S = S"
   unfolding edge_collect_def by (auto split: if_splits)
 
 lemma edge_collect_single:
