src/Examples/Interval/Example_Interval_DG_Flagship.thy
@@ -228,7 +228,9 @@ proof -
              flagship_ex_transfer.tf_sound_enter_for flagship_ex_transfer.tf_sound_combine_for
              ivl_tf_st_for_commute[folded fun_of_exec_dg_st_for_def]
              ivl_enter_st_for_commute[folded fun_of_exec_dg_st_for_def]
-             ivl_tf_st_for_ret_None ivl_tf_st_for_ret_Some
+             action_reduces.ret_none[OF ivl_tf_st_for_reduces]
+             action_reduces.ret_some[OF ivl_tf_st_for_reduces]
+             action_reduces.check[OF ivl_tf_st_for_reduces]
              TD_side_warrowing_apinis_Interp.part_post_solution_of_solve_c)+
 qed
 
